Proof on Spec

Rocq/src/Spec.v
@@ -13,61 +13,27 @@ Import Utils.
 Set Implicit Arguments.
 
 Module Spec.
+
   Section SpecDef.
-    Variable pass1 : Expr -> path -> nat.
+    Fixpoint pass1 e :=
+      match e with
+      | EAtom op => op
+      | EBinOp lhs rhs => max (pass1 lhs) (pass1 rhs)
+      | EUnOp arg => pass1 arg
+      | ECast arg => pass1 arg
+      | EComp _ _ => 1
+      | ELogic _ _ => 1
+      | EReduction _ => 1
+      | EShift lhs _ => pass1 lhs
+      | EAssign lval _ => lval
+      | EShiftAssign lval _ => lval
+      | ECond _ lhs rhs => max (pass1 lhs) (pass1 rhs)
+      | EConcat args => sum (map pass1 args)
+      | ERepl i arg => i * pass1 arg
+      end
+    .
+
     Variable pass2 : Expr -> path -> nat.
-
-    Definition atom_pass1 :=
-      forall e p op, e @[p] = Some (EAtom op) -> pass1 e p = op.
-
-    Definition binop_pass1 :=
-      forall e p lhs rhs,
-        e @[p] = Some (EBinOp lhs rhs) ->
-        pass1 e p = max (pass1 e (p ++ [Lhs])) (pass1 e (p ++ [Rhs])).
-
-    Definition unop_pass1 :=
-      forall e p arg, e @[p] = Some (EUnOp arg) -> pass1 e p = pass1 e (p ++ [Arg]).
-
-    Definition cast_pass1 :=
-      forall e p arg, e @[p] = Some (ECast arg) -> pass1 e p = pass1 e (p ++ [Arg]).
-
-    Definition comp_pass1 :=
-      forall e p lhs rhs, e @[p] = Some (EComp lhs rhs) -> pass1 e p = 1.
-
-    Definition logic_pass1 :=
-      forall e p lhs rhs, e @[p] = Some (ELogic lhs rhs) -> pass1 e p = 1.
-
-    Definition red_pass1 :=
-      forall e p arg, e @[p] = Some (EReduction arg) -> pass1 e p = 1.
-
-    Definition shift_pass1 :=
-      forall e p lhs rhs, e @[p] = Some (EShift lhs rhs) -> pass1 e p = pass1 e (p ++ [Lhs]).
-
-    Definition assign_pass1 :=
-      forall e p lval arg, e @[p] = Some (EAssign lval arg) -> pass1 e p = lval.
-
-    Definition shiftassign_pass1 :=
-      forall e p lval arg, e @[p] = Some (EShiftAssign lval arg) -> pass1 e p = lval.
-
-    Definition cond_pass1 :=
-      forall e p cond lhs rhs,
-        e @[p] = Some (ECond cond lhs rhs) ->
-        pass1 e p = max (pass1 e (p ++ [Lhs])) (pass1 e (p ++ [Rhs])).
-
-    Definition concat_pass1 :=
-      forall e p args pList,
-        e @[p] = Some (EConcat args) ->
-        (forall i, nth_error pList i = Some (pass1 e (p ++ [Args i]))) ->
-        pass1 e p = sum pList.
-
-    Definition repl_pass1 :=
-      forall e p i arg, e @[p] = Some (ERepl i arg) -> pass1 e p = i * pass1 e (p ++ [Arg]).
-
-
-
-    Definition sd e p := pass2 e p = pass1 e p.
-
-
 
     Definition binop_pass2 :=
       forall e p lhs rhs,
@@ -78,57 +44,129 @@ Module Spec.
       forall e p arg, e @[p] = Some (EUnOp arg) -> pass2 e (p ++ [Arg]) = pass2 e p.
 
     Definition cast_pass2 :=
-      forall e p arg, e @[p] = Some (ECast arg) -> sd e (p ++ [Arg]).
+      forall e p arg, e @[p] = Some (ECast arg) -> pass2 e (p ++ [Arg]) = pass1 arg.
 
     Definition comp_pass2 :=
       forall e p lhs rhs,
         e @[p] = Some (EComp lhs rhs) ->
-        forall s, s = max (pass1 e (p ++ [Lhs])) (pass1 e (p ++ [Rhs])) ->
+        forall s, s = max (pass1 lhs) (pass1 rhs) ->
              pass2 e (p ++ [Lhs]) = s /\ pass2 e (p ++ [Rhs]) = s.
 
     Definition logic_pass2 :=
       forall e p lhs rhs,
-        e @[p] = Some (ELogic lhs rhs) -> sd e (p ++ [Lhs]) /\ sd e (p ++ [Rhs]).
+        e @[p] = Some (ELogic lhs rhs) -> pass2 e (p ++ [Lhs]) = pass1 lhs /\ pass2 e (p ++ [Rhs]) = pass1 rhs.
 
     Definition red_pass2 :=
-      forall e p arg, e @[p] = Some (EReduction arg) -> sd e (p ++ [Arg]).
+      forall e p arg, e @[p] = Some (EReduction arg) -> pass2 e (p ++ [Arg]) = pass1 arg.
 
     Definition shift_pass2 :=
       forall e p lhs rhs, e @[p] = Some (EShift lhs rhs) ->
-                     sd e (p ++ [Rhs]) /\ pass2 e (p ++ [Lhs]) = pass2 e p.
+                     pass2 e (p ++ [Lhs]) = pass2 e p /\ pass2 e (p ++ [Rhs]) = pass1 rhs.
 
     Definition assign_pass2 :=
       forall e p lval arg,
         e @[p] = Some (EAssign lval arg) ->
-        forall s, s = max (pass1 e (p ++ [Arg])) lval -> pass2 e (p ++ [Arg]) = s.
+        forall s, s = max (pass1 arg) lval -> pass2 e (p ++ [Arg]) = s.
 
     Definition shiftassign_pass2 :=
-      forall e p lval arg, e @[p] = Some (EShiftAssign lval arg) -> sd e (p ++ [Arg]).
+      forall e p lval arg, e @[p] = Some (EShiftAssign lval arg) -> pass2 e (p ++ [Arg]) = pass1 arg.
 
     Definition cond_pass2 :=
       forall e p cond lhs rhs,
         e @[p] = Some (ECond cond lhs rhs) ->
         pass2 e (p ++ [Lhs]) = pass2 e p /\ pass2 e (p ++ [Rhs]) = pass2 e p /\
-          sd e (p ++ [Cond]).
+          pass2 e (p ++ [Cond]) = pass1 cond.
 
     Definition concat_pass2 :=
       forall e p args, e @[p] = Some (EConcat args) ->
-                  forall i, i < length args -> sd e (p ++ [Args i]).
+                  forall i f, nth_error args i = Some f -> pass2 e (p ++ [Args i]) = pass1 f.
 
     Definition repl_pass2 :=
-      forall e p i arg, e @[p] = Some (ERepl i arg) -> sd e (p ++ [Arg]).
+      forall e p i arg, e @[p] = Some (ERepl i arg) -> pass2 e (p ++ [Arg]) = pass1 arg.
 
-    Definition pass1_def :=
-      atom_pass1 /\ binop_pass1 /\ unop_pass1 /\ cast_pass1 /\
-        comp_pass1 /\ logic_pass1 /\ red_pass1 /\ shift_pass1 /\
-        assign_pass1 /\ shiftassign_pass1 /\ cond_pass1 /\ concat_pass1 /\
-        repl_pass1.
+    Definition toplevel_pass2 := forall e, pass2 e [] = pass1 e.
 
     Definition pass2_def :=
-      binop_pass2 /\ unop_pass2 /\ cast_pass2 /\ comp_pass2 /\
-        logic_pass2 /\ red_pass2 /\ shift_pass2 /\ assign_pass2 /\
-        shiftassign_pass2 /\ cond_pass2 /\ concat_pass2 /\ repl_pass2.
-
-    Definition pass_def := pass1_def /\ pass2_def.
+      toplevel_pass2 /\ binop_pass2 /\ unop_pass2 /\ cast_pass2 /\
+        comp_pass2 /\ logic_pass2 /\ red_pass2 /\ shift_pass2 /\
+        assign_pass2 /\ shiftassign_pass2 /\ cond_pass2 /\
+        concat_pass2 /\ repl_pass2.
   End SpecDef.
+
+  Theorem pass2_val : forall p e, IsPath e p -> forall f, pass2_def f -> exists n, f e p = n.
+  Proof.
+    induction p using path_ind; intros.
+    - firstorder.
+    - assert (He: IsPath e p /\ exists f, e @[p] = Some f /\ IsPath f [x]).
+      + split. apply (IsPath_prefix _ _ H). apply IsPath_chunk. assumption.
+      + destruct He as [H1 [expr [H2 H3]]].
+        destruct expr; inv H3; destruct (IHp _ H1 _ H0); try (eexists; firstorder).
+  Qed.
+
+  Ltac pass2_def_split :=
+    match goal with
+    | [ H: pass2_def _ |- _ ] =>
+        destruct H as [?HTopLevel [?HBinOp [?HUnOp [?HCast [?HComp [?HLogic [?HRed [?HShift [?HAssign [?HShiftAssign [?HCond [?HConcat ?HRepl]]]]]]]]]]]]
+    end
+  .
+
+  Theorem pass2_unique : forall p e,
+      IsPath e p -> forall f1 f2, pass2_def f1 -> pass2_def f2 -> f1 e p = f2 e p.
+  Proof.
+    Ltac _pass2_unique_tac :=
+      match goal with
+      | [ G: _ _ _ = _ _ _, F: _ @[_] = Some (EBinOp _ _), H: binop_pass2 _ |- _ ] =>
+          destruct (H _ _ _ _ F); rewrite G in *; assumption
+      | [ G: _ _ _ = _ _ _, F: _ @[_] = Some (EUnOp _), H: unop_pass2 _ |- _ ] =>
+          apply H in F; rewrite G in *; assumption
+      | [ F: _ @[_] = Some (ELogic _ _), H: logic_pass2 _ |- _ ] =>
+          destruct (H _ _ _ _ F); assumption
+      | [ F: _ @[_] = Some (EReduction _), H: red_pass2 _ |- _ ] =>
+          apply H in F; assumption
+      | [ G: _ _ _ = _ _ _, F: _ @[_] = Some (EShift _ _), H: shift_pass2 _ |- _ ] =>
+          destruct (H _ _ _ _ F); assumption || rewrite G in *; assumption
+      | [ F: _ @[_] = Some (EAssign _ _), H: assign_pass2 _ |- _ ] =>
+          apply (H _ _ _ _ F); reflexivity
+      | [ F: _ @[_] = Some (EShiftAssign _ _), H: shiftassign_pass2 _ |- _ ] =>
+          apply (H _ _ _ _ F)
+      | [ G: _ _ _ = _ _ _, F: _ @[_] = Some (ECond _ _ _), H: cond_pass2 _ |- _ ] =>
+          destruct (H _ _ _ _ _ F) as [? []]; assumption || rewrite G in *; assumption
+      | [ G: nth_error _ _ = _, F: _ @[_] = Some (EConcat _), H: concat_pass2 _ |- _ ] =>
+          apply (H _ _ _ F _ _ G)
+      | [ F: _ @[_] = Some (ERepl _ _), H: repl_pass2 _ |- _ ] =>
+          apply (H _ _ _ _ F)
+      end
+    .
+    assert (Heq: forall x y m : nat, x = m -> y = m -> x = y). { intros. subst. reflexivity. }
+    induction p using path_ind; intros.
+    - apply eq_trans with (y := pass1 e). firstorder. symmetry. firstorder.
+    - assert (He: IsPath e p /\ exists f, e @[p] = Some f /\ IsPath f [x]).
+      + split. apply (IsPath_prefix _ _ H). apply IsPath_chunk. assumption.
+      + destruct He as [H2 [expr [H3 H4]]].
+        assert (Hf: f1 e p = f2 e p). apply (IHp _ H2 _ _ H0 H1). clear IHp.
+        destruct expr; inv H4; repeat pass2_def_split.
+        * apply Heq with (m := f1 e p); _pass2_unique_tac.
+        * apply Heq with (m := f1 e p); _pass2_unique_tac.
+        * apply Heq with (m := f1 e p); _pass2_unique_tac.
+        * apply Heq with (m := pass1 expr); firstorder.
+        * apply Heq with (m := max (pass1 expr1) (pass1 expr2)).
+          destruct (HComp0 _ _ _ _ H3 (max (pass1 expr1) (pass1 expr2))); auto.
+          destruct (HComp _ _ _ _ H3 (max (pass1 expr1) (pass1 expr2))); auto.
+        * apply eq_trans with (y := max (pass1 expr1) (pass1 expr2)).
+          destruct (HComp0 _ _ _ _ H3 (max (pass1 expr1) (pass1 expr2))); auto.
+          destruct (HComp _ _ _ _ H3 (max (pass1 expr1) (pass1 expr2))); auto.
+        * apply Heq with (m := pass1 expr1); _pass2_unique_tac.
+        * apply Heq with (m := pass1 expr2); _pass2_unique_tac.
+        * apply Heq with (m := pass1 expr); _pass2_unique_tac.
+        * apply Heq with (m := f1 e p); _pass2_unique_tac.
+        * apply Heq with (m := pass1 expr2); _pass2_unique_tac.
+        * apply Heq with (m := max (pass1 expr) lval); _pass2_unique_tac.
+        * apply Heq with (m := pass1 expr); _pass2_unique_tac.
+        * apply Heq with (m := pass1 expr1); _pass2_unique_tac.
+        * apply Heq with (m := f1 e p); _pass2_unique_tac.
+        * apply Heq with (m := f1 e p); _pass2_unique_tac.
+        * apply Heq with (m := pass1 e0); _pass2_unique_tac.
+        * apply Heq with (m := pass1 expr); _pass2_unique_tac.
+  Qed.
+
 End Spec.
